False axiom

RBEP_IOvsState.v
@@ -400,12 +400,12 @@ Definition EE' := forall be t,
     ndeval' be t <-> steval' (proj_input t) be (proj_output t).
 Conjecture lang_is_EE' : EE'.
 
-Definition REP_IO :=
+Definition BEP_IO :=
   forall be1 be2,
     (forall t, ndeval be1 t <-> ndeval be2 t) ->
     (forall t, ndeval' (compile be1) t <-> ndeval' (compile be2) t).
 
-Definition REP_State :=
+Definition BEP_State :=
   forall be1 be2 is1 is2,
     (* Input stream quantified at highest level, as if it were part of the program *)
     (forall os, steval is1 be1 os <-> steval is2 be2 os) ->
@@ -420,9 +420,9 @@ Proof.
   tauto.
 Qed.
 
-Lemma conjecture4 : REP_State -> REP_IO.
+Lemma conjecture4 : BEP_State -> BEP_IO.
 Proof.
-  unfold REP_State, REP_IO.
+  unfold BEP_State, BEP_IO.
   intros H be1 be2 H0.
   assert (H' : forall (be1 be2 : bexp) (is1 : stream bool),
              (forall os : trace output,
